<rdf:RDF
    xmlns:rdf="http://www.w3.org/1999/02/22-rdf-syntax-ns#"
    xmlns:owl="http://www.w3.org/2002/07/owl#"
    xmlns:rdfs="http://www.w3.org/2000/01/rdf-schema#"
    xmlns="http://swlab.ic.uff.br/ontology/EntityRelatednessTestData_v1.rdf#">
  <rdfs:Class rdf:about="http://swlab.ic.uff.br/ontology/EntityRelatednessTestData_v1.rdf#EntityPair">
    <rdfs:comment>A pair of entities for which one want to findconnectivity profiles.</rdfs:comment>
    <rdfs:label>EntityPair</rdfs:label>
  </rdfs:Class>
  <rdfs:Class rdf:about="http://swlab.ic.uff.br/ontology/EntityRelatednessTestData_v1.rdf#ListOfPathElements">
    <rdfs:comment>The container of the elements of a path.</rdfs:comment>
    <rdfs:label>ListOfPathElements</rdfs:label>
    <rdfs:subClassOf rdf:resource="http://www.w3.org/1999/02/22-rdf-syntax-ns#List"/>
  </rdfs:Class>
  <rdfs:Class rdf:about="http://swlab.ic.uff.br/ontology/EntityRelatednessTestData_v1.rdf#PropertyElement">
    <rdfs:comment>A property of a path.</rdfs:comment>
    <rdfs:label>PropertyElement</rdfs:label>
    <rdfs:subClassOf>
      <rdfs:Class rdf:about="http://swlab.ic.uff.br/ontology/EntityRelatednessTestData_v1.rdf#PathElement"/>
    </rdfs:subClassOf>
  </rdfs:Class>
  <rdfs:Class rdf:about="http://swlab.ic.uff.br/ontology/EntityRelatednessTestData_v1.rdf#Entity">
    <rdfs:comment>A knowledge base B is a set of RDF triples. We say that an entity of B is a URI that occurs as a subject or object of a triple in B.</rdfs:comment>
    <rdfs:label>Entity</rdfs:label>
  </rdfs:Class>
  <rdfs:Class rdf:about="http://swlab.ic.uff.br/ontology/EntityRelatednessTestData_v1.rdf#Path">
    <rdfs:comment>A path Ï€ of a knowledge base B is an undirected path in the graph GB induced by B. The notions of start node and end node of a path are defined as usual. Note that, by considering an undirected path, we allow the edges of the RDF graph to be reversely traversed.</rdfs:comment>
    <rdfs:label>Path</rdfs:label>
  </rdfs:Class>
  <rdfs:Class rdf:about="http://swlab.ic.uff.br/ontology/EntityRelatednessTestData_v1.rdf#EntityElement">
    <rdfs:comment>An entity of a path.</rdfs:comment>
    <rdfs:label>EntityElement</rdfs:label>
    <rdfs:subClassOf>
      <rdfs:Class rdf:about="http://swlab.ic.uff.br/ontology/EntityRelatednessTestData_v1.rdf#PathElement"/>
    </rdfs:subClassOf>
  </rdfs:Class>
  <rdfs:Class rdf:about="http://swlab.ic.uff.br/ontology/EntityRelatednessTestData_v1.rdf#PathElement">
    <rdfs:comment>The elements (entities and properties) of a path.</rdfs:comment>
    <rdfs:label>PathElement</rdfs:label>
  </rdfs:Class>
  <rdf:Description rdf:about="http://swlab.ic.uff.br/ontology/EntityRelatednessTestData_v1.rdf#score">
    <rdfs:domain rdf:resource="http://swlab.ic.uff.br/ontology/EntityRelatednessTestData_v1.rdf#PathElement"/>
    <rdfs:comment>The rank score of a path with respect to a pair of entities.</rdfs:comment>
    <rdfs:label>score</rdfs:label>
    <rdfs:range rdf:resource="http://www.w3.org/2001/XMLSchema#double"/>
    <rdfs:domain rdf:resource="http://swlab.ic.uff.br/ontology/EntityRelatednessTestData_v1.rdf#Path"/>
  </rdf:Description>
  <rdf:Description rdf:about="http://swlab.ic.uff.br/ontology/EntityRelatednessTestData_v1.rdf#">
    <owl:versionInfo>0.1</owl:versionInfo>
  </rdf:Description>
  <rdf:Description rdf:about="http://swlab.ic.uff.br/ontology/EntityRelatednessTestData_v1.rdf#hasListOfpathElements">
    <rdfs:comment>The relationship between a path and a list of path elements.</rdfs:comment>
    <rdfs:label>hasListOfpathElements</rdfs:label>
    <rdfs:range rdf:resource="http://swlab.ic.uff.br/ontology/EntityRelatednessTestData_v1.rdf#ListOfPathElements"/>
    <rdfs:domain rdf:resource="http://swlab.ic.uff.br/ontology/EntityRelatednessTestData_v1.rdf#Path"/>
  </rdf:Description>
  <rdf:Description rdf:about="http://swlab.ic.uff.br/ontology/EntityRelatednessTestData_v1.rdf#first">
    <rdfs:comment>The first element of a list of path elements.</rdfs:comment>
    <rdfs:label>first</rdfs:label>
    <rdfs:range rdf:resource="http://swlab.ic.uff.br/ontology/EntityRelatednessTestData_v1.rdf#PathElement"/>
    <rdfs:domain rdf:resource="http://swlab.ic.uff.br/ontology/EntityRelatednessTestData_v1.rdf#ListOfPathElements"/>
    <rdfs:subPropertyOf rdf:resource="http://www.w3.org/1999/02/22-rdf-syntax-ns#first"/>
  </rdf:Description>
  <rdf:Description rdf:about="http://swlab.ic.uff.br/ontology/EntityRelatednessTestData_v1.rdf#entity">
    <rdfs:comment>A reference to an erel:Entity.</rdfs:comment>
    <rdfs:label>entity</rdfs:label>
    <rdfs:range rdf:resource="http://swlab.ic.uff.br/ontology/EntityRelatednessTestData_v1.rdf#Entity"/>
    <rdfs:domain rdf:resource="http://swlab.ic.uff.br/ontology/EntityRelatednessTestData_v1.rdf#EntityElement"/>
  </rdf:Description>
  <rdf:Description rdf:about="http://swlab.ic.uff.br/ontology/EntityRelatednessTestData_v1.rdf#entity2">
    <rdfs:comment>The second entity of a pair of entities.</rdfs:comment>
    <rdfs:label>entity2</rdfs:label>
    <rdfs:range rdf:resource="http://swlab.ic.uff.br/ontology/EntityRelatednessTestData_v1.rdf#Entity"/>
    <rdfs:domain rdf:resource="http://swlab.ic.uff.br/ontology/EntityRelatednessTestData_v1.rdf#EntityPair"/>
  </rdf:Description>
  <rdf:Description rdf:about="http://swlab.ic.uff.br/ontology/EntityRelatednessTestData_v1.rdf#entity1">
    <rdfs:comment>The first entity of a pair of entities.</rdfs:comment>
    <rdfs:label>entity1</rdfs:label>
    <rdfs:range rdf:resource="http://swlab.ic.uff.br/ontology/EntityRelatednessTestData_v1.rdf#Entity"/>
    <rdfs:domain rdf:resource="http://swlab.ic.uff.br/ontology/EntityRelatednessTestData_v1.rdf#EntityPair"/>
  </rdf:Description>
  <rdf:Description rdf:about="http://swlab.ic.uff.br/ontology/EntityRelatednessTestData_v1.rdf#rest">
    <rdfs:comment>The remaining elements of a list of path elelements.</rdfs:comment>
    <rdfs:label>rest</rdfs:label>
    <rdfs:range rdf:resource="http://swlab.ic.uff.br/ontology/EntityRelatednessTestData_v1.rdf#ListOfPathElements"/>
    <rdfs:domain rdf:resource="http://swlab.ic.uff.br/ontology/EntityRelatednessTestData_v1.rdf#ListOfPathElements"/>
    <rdfs:subPropertyOf rdf:resource="http://www.w3.org/1999/02/22-rdf-syntax-ns#rest"/>
  </rdf:Description>
  <rdf:Description rdf:about="http://swlab.ic.uff.br/ontology/EntityRelatednessTestData_v1.rdf#property">
    <rdfs:comment>A reference to an rdf:Property.</rdfs:comment>
    <rdfs:label>property</rdfs:label>
    <rdfs:range rdf:resource="http://www.w3.org/1999/02/22-rdf-syntax-ns#Property"/>
    <rdfs:domain rdf:resource="http://swlab.ic.uff.br/ontology/EntityRelatednessTestData_v1.rdf#PropertyElement"/>
  </rdf:Description>
  <rdf:Description rdf:about="http://swlab.ic.uff.br/ontology/EntityRelatednessTestData_v1.rdf#hasPath">
    <rdfs:comment>The relationship between a pair of entities and a path.The set of all paths of a pair of entities make up the rank list of relevant paths between the pair of entities.</rdfs:comment>
    <rdfs:label>hasPath</rdfs:label>
    <rdfs:range rdf:resource="http://swlab.ic.uff.br/ontology/EntityRelatednessTestData_v1.rdf#Path"/>
    <rdfs:domain rdf:resource="http://swlab.ic.uff.br/ontology/EntityRelatednessTestData_v1.rdf#EntityPair"/>
  </rdf:Description>
  <rdf:Description rdf:about="http://swlab.ic.uff.br/ontology/EntityRelatednessTestData_v1.rdf#position">
    <rdfs:comment>The position of the element in the path.</rdfs:comment>
    <rdfs:label>position</rdfs:label>
    <rdfs:range rdf:resource="http://www.w3.org/2001/XMLSchema#int"/>
    <rdfs:domain rdf:resource="http://swlab.ic.uff.br/ontology/EntityRelatednessTestData_v1.rdf#PathElement"/>
  </rdf:Description>
  <rdf:Description rdf:about="http://swlab.ic.uff.br/ontology/EntityRelatednessTestData_v1.rdf#expression">
    <rdfs:comment>The label of a path.</rdfs:comment>
    <rdfs:label>expression</rdfs:label>
    <rdfs:range rdf:resource="http://www.w3.org/2001/XMLSchema#string"/>
    <rdfs:domain rdf:resource="http://swlab.ic.uff.br/ontology/EntityRelatednessTestData_v1.rdf#Path"/>
  </rdf:Description>
  <rdf:Description rdf:about="http://swlab.ic.uff.br/ontology/EntityRelatednessTestData_v1.rdf#rank">
    <rdfs:comment>The rank position of a path with respect to a pair of entities.</rdfs:comment>
    <rdfs:label>rank</rdfs:label>
    <rdfs:range rdf:resource="http://www.w3.org/2001/XMLSchema#long"/>
    <rdfs:domain rdf:resource="http://swlab.ic.uff.br/ontology/EntityRelatednessTestData_v1.rdf#Path"/>
  </rdf:Description>
</rdf:RDF>
